# Unwrapped - Sum of Sinusoids [7:28]
* Assume we start with $A_1e^{j(\omega t+ \phi_1)} + A_2e^{j(\omega t+\phi_2)}$
	* We can break this up into $A_1e^{j\omega t}e^{j\phi_1} + A_2e^{j\omega t}e^{j\phi_2}$
	* This can be further simplified into $e^{j\omega t} [A_1e^{j\phi_1}+A_2e^{j\phi_2}]$
	* ![[Pasted image 20250121203839.png]]
	* The basic idea is to take the magnitude of each vector, and add it like you would, to get the resulting Re and Im parts of the combined complex sinusoid. 
	* Returning back the $e^{j\omega t}$ we get our original form back after summing 2 sinusoids

# Sum of Sinusoids 1 (Wong) [49:12]
* "Inverse" Euler's Formula**s**
	* $cos(\theta) = \frac{e^{j\theta} + e^{-j\theta}}{2}$
	* $sin(\theta) = \frac{e^{j\theta} - e^{-j\theta}}{2j}$
* Negative Frequency is a LIE
	* $Acos(\omega_0t+\phi)$  
	* $= \frac{A}{2}e^{j\phi}e^{j\omega_0t} + \frac{A}{2}e^{-j\phi}e^{-j\omega_0t}$
	*  If we add up the first phasor $\frac{A}{2}e^{j\phi}$ with it's complex conjugate $\frac{A}{2}e^{-j\phi}$, and the two frequencies have opposite values ($j\omega_0t$ & $-j\omega_0t$), we will return the positive frequency real sinusoid!
	* Negative frequency is the same as positive frequency in the real world, so we use the above mathematical tool to convert a negative frequency into a positive one, with the complex conjugates of the phasors
	* ![[Pasted image 20250121211405.png]]
* Example:
	* $$x(t) = 10 + 14cos(200\pi t - \frac{\pi}{3}) + 8cos(500\pi t + \frac{\pi}{2})$$
	* Let's throw this into `MATLAB` 
```R
function [s,t]=sinu(A,f0,phi,fs,n)

Ts=1/fs;
t=[0:Ts:(n-1)*Ts];
s=A*cos(2*pi*f0*t+phi);

end
``` 

```R
edit sinu.m
[x2, t] = sinu(14,100,-pi/3,8000,8000);
plot(t, x2)

clear all
[x2, t] = sinu(14,100,-pi/3,8000,8000);
plot(t, x2)
soundsc(x2, 8000)
x1 = sinu(10,0,0,8000,8000);
x3 = sinu(8,250,pi/2,8000,8000);
soundsc(x3, 8000);
x = x1 + x2 + x3; # IF not the same length, matlab won't add them.
plot(t, x)
```

* The sum of the three sinusoinds ends up becoming **NOT** a sinusoid. We know that we only get a sinusoid back when all the frequencies are the same. 
* Now, let's do it with algebra, using inverse euler's formulas
	* $10 + 7e^{+j\frac{pi}{3}}e^{-j200\pi t} + 7e^{-j\frac{pi}{3}}e^{j200\pi t} + 4e^{-j\frac{\pi}{2}}e^{-j500\pi t} + 4e^{j\frac{\pi}{2}}e^{j500\pi t}$
	* I ain't typing all that
	  ![[Pasted image 20250121224135.png]]
	  * ![[Pasted image 20250121224419.png]]Basically, this is just saying adding them all up returns the original complex sinusoidal. 
# Sum of Sinusoids 2 [54:09]
* $x(t) = A_0 + \Sigma_{i=1}^{N} A_icos(2\pi f_it + \phi_i); \space f_1 = k_if_0\space where\space k_1,\space k_2\space,...,\space k_N\space are\space positive\space integers\space and\space gcd\space(k_1,k_2,...,k_N) = 1$
* then, x(t) is periodic with $T_0 = \frac{1}{f_0};\space f_0 = fundamental \space freq.$ 
* $x(t) = A_0 t \Sigma_{i = 1}^{N} (\frac{A_i}{2}e^{j\phi_i}e^{j2\pi k_i f_0 t} + \frac{A_i}{2}e^{-j\phi_i}e^{-j2\pi k_i f_0 t})$
* $= \Sigma_{k = -M}^{M} (a_k e^{j2\pi k f_0t})$ 
* ![[Pasted image 20250121225321.png]]
	* This situation is the only way you get back a periodic signal when summing up n-complex sinusoids.
* Example:
	* $x(t) = 10 + 14cos(200\pi t- \frac{\pi}{3}) + 8cos(500\pi t + \frac{\pi}{2}) + 6cos(600\pi t)$ 
		* $f_1 = 100 = 2 * 50$
		* $f_2 = 250 = 5 * 50$
		* $f_3 = 300 = 6 * 50$
		* $gcd(2,5,6) = 1$
		* $50 = fundamental \space frequency$
		* idk what wong is on about, but uhhh make sure the condition is met so they return a periodic sinusoid.
* Example:
	* $x(t) = cos(2\pi f_1 t) + cos(2\pi f_2 t)$ where $f_1 = f_c - \triangle$    and $f_2 = f_c t \triangle$ $(f_c = \frac{1}{2}(f_1 + f_2) = center \space frequency)$ and $\triangle = \frac{1}{2}(f_2 - f_1) = frequency \space deviation.$ so, $f_c = k\triangle ; \space k \space large \space integer$  
* I've stopped caring about Wong's proofs.
* Example:
	* ![[Pasted image 20250122220914.png]]
	* ![[Pasted image 20250122220936.png]]
	* i'm done with wong's ramblings in this vid.

# Fourier Series 1 [9:43]
* $x(t) = A_1e^{-j(\frac{\pi}{2} t+ \phi_1)} + A_2e^{-j(\frac{\pi}{3} t+\phi_2)}$ 
	* $c = A_1e^{-j\phi_1}$
	* $c = A_2e^{-j\phi_2}$
	* what about are indeces?
	* let's determine a fundamental frequency $f_0 = \frac{\pi}{6}$ 
		* $f_0 * -2 = \frac{\pi}{3}$
		* $f_0 * -3 = \frac{\pi}{2}$ 
	* Now they become
		* $c_{-3} = A_1e^{-j\phi_1}$
		* $c_{-2} = A_2e^{-j\phi_2}$
* ![[Pasted image 20250122224454.png]]
# Fourier Series 1 [37:34]
* Fourier Series
	* Extension of what we've already done
	* "Almost all" periodic signals can be generated by adding up harmonics together. 
	* Equation (ignoring mathematical exceptions):
		* $x(t) = \Sigma_{k = -\infty}^{\infty} (a_ke^{j\frac{2\pi kt}{T_0}})$ 
		* $x(t) = x(t + t_0)$ 
		* ![[Pasted image 20250122225405.png]]
	* To synthesis a Fourier series is easy, basically depends how powerful your computer is. From frequency domain to time domain.
	* Analyzing a Fourier series is hard, from time domain to frequency domain.
* Orthogonality of harmonics
	* ![[Pasted image 20250122230728.png]]
	* * = conjugate
	* We're multiplying a sinusoid and a conjugate of another and integrating it over 1 period. 
	* ![[Pasted image 20250122231124.png]]
	* Big nothingburger again

# Thursday Class 1/23
* Explaining HW
* $x^3 = 8; (2e^{\pm j\frac{2\pi}{3}})^3 = 8e^{\pm j2\pi} = 8 = -1 \pm \sqrt{3}$   
```
  joel "i go both ways" harley
```

